% Equation 1
\begin{dmath}
{Y^s_{t}}={C^s_{t}}+{DB^b_{t}}+{TB^s_{t}}
\end{dmath}
% Equation 2
\begin{dmath}
{Y^s_{t}}={w_{t}}\, {L^s_{t}}+{\Pi^{local}_{banks}_{t}}+{ Gift From Borrowers _{t}}
\end{dmath}
% Equation 3
\begin{dmath}
{ Gift From Borrowers _{t}}=\frac{{\chi^b }\, { NetWorth_b _{t}}}{{chi\_s}}\, \left({ Net Worth Shock _{t}}-1\right)
\end{dmath}
% Equation 4
\begin{dmath}
{ Net Worth Shock _{t}}={ Net Worth Shock _{t-1}}^{{\rho(e^NW) }}\, exp\left({e\_NW_{t}}\, {\sigma(e^NW) }\right)
\end{dmath}
% Equation 5
\begin{dmath}
{\Pi^{local}_{banks}_{t}}=\left(-{b^s_{t}}\right)\, \left(\frac{1}{{ R^s_{nom}_{t}}}-\frac{1}{{ R^b_{nom}_{t}}}\right)
\end{dmath}
% Equation 6
\begin{dmath}
{DB^b_{t}}=\frac{{b^b_{t-1}}}{{ \Pi _{t}}}-\frac{{b^b_{t}}}{{ R^b_{nom}_{t}}}
\end{dmath}
% Equation 7
\begin{dmath}
{DB^b_{t}}=\frac{{b^s_{t-1}}}{{ \Pi _{t}}}-\frac{{b^s_{t}}}{{ R^s_{nom}_{t}}}
\end{dmath}
% Equation 8
\begin{dmath}
{TB^b_{t}}={b^{b*}_{t-1}}-\frac{{b^{b*}_{t}}}{{R^{b*}_{t}}}
\end{dmath}
% Equation 9
\begin{dmath}
{TB^s_{t}}={b^{s*}_{t-1}}-\frac{{b^{s*}_{t}}}{{R^{s*}_{t}}}
\end{dmath}
% Equation 10
\begin{dmath}
{\delta _{t}}={ p \delta }^{1-{ \rho(e^{\delta}) }}\, {\delta _{t-1}}^{{ \rho(e^{\delta}) }}\, exp\left({e\_delta_{t}}\, { \sigma(e^{\delta}) }\right)
\end{dmath}
% Equation 11
\begin{dmath}
{K_b_{t}}={I^b_{t-1}}+\left(1-{\delta _{t}}\right)\, {K_b_{t-1}}
\end{dmath}
% Equation 12
\begin{dmath}
{\{mu}^b_{t}}=\left({C^b_{t}}-{h^b }\, {C^b_{t-1}}\right)^{\left(-{sigma\_b}\right)}-{h^b }\, {beta\_b}\, \left({C^b_{t+1}}-{C^b_{t}}\, {h^b }\right)^{\left(-{sigma\_b}\right)}
\end{dmath}
% Equation 13
\begin{dmath}
{\{mu}^s_{t}}=\left({C^s_{t}}-{h^s }\, {C^s_{t-1}}\right)^{\left(-{\sigma_s}\right)}-{h^s }\, {\beta_s}\, \left({C^s_{t+1}}-{C^s_{t}}\, {h^s }\right)^{\left(-{\sigma_s}\right)}
\end{dmath}
% Equation 14
\begin{dmath}
{\{mu}^{REP}_{t}}=\left({C_{t}}-{h^s }\, {C_{t-1}}\right)^{\left(-{\sigma_s}\right)}-{h^s }\, {\beta_s}\, \left({C_{t+1}}-{h^s }\, {C_{t}}\right)^{\left(-{\sigma_s}\right)}
\end{dmath}
% Equation 15
\begin{dmath}
{w_{t}}=\frac{{\vartheta^b}\, {L^b_{t}}^{{\omega^b }}}{{\{mu}^b_{t}}}
\end{dmath}
% Equation 16
\begin{dmath}
{w_{t}}=\frac{{\vartheta^s}\, {L^s_{t}}^{{\omega^s }}}{{\{mu}^s_{t}}}
\end{dmath}
% Equation 17
\begin{dmath}
{ m_b _{t}}=\frac{{\{mu}^b_{t}}\, {beta\_b}}{{\{mu}^b_{t-1}}}
\end{dmath}
% Equation 18
\begin{dmath}
{ m_s _{t}}=\frac{{\{mu}^s_{t}}\, {\beta_s}}{{\{mu}^s_{t-1}}}
\end{dmath}
% Equation 19
\begin{dmath}
{ m_REP _{t}}=\frac{{\beta_s}\, {\{mu}^{REP}_{t}}}{{\{mu}^{REP}_{t-1}}}
\end{dmath}
% Equation 20
\begin{dmath}
{ R_k _{t}}=\frac{{q_{t+1}}+\left(1-{\delta _{t}}\right)\, { Q_k _{t+1}}}{{ Q_k _{t}}}
\end{dmath}
% Equation 21
\begin{dmath}
{I_{AC}_{t}}=\frac{{\gamma_2_b}}{2}\, \left(\frac{{I_{t}}}{{I_{t-1}}}-1\right)^{2}
\end{dmath}
% Equation 22
\begin{dmath}
{I_{MC}_{t}}={\gamma_2_b}\, \left(\frac{{I_{t}}}{{I_{t-1}}}-1\right)
\end{dmath}
% Equation 23
\begin{dmath}
{ R_i _{t}}=\frac{1}{{beta\_b}}
\end{dmath}
% Equation 24
\begin{dmath}
{ Q_k _{t}}=1+{I_{AC}_{t}}+\frac{{I_{t}}}{{I_{t-1}}}\, {I_{MC}_{t}}-{ m_b _{t+1}}\, {I_{MC}_{t+1}}\, \left(\frac{{I_{t+1}}}{{I_{t}}}\right)^{2}
\end{dmath}
% Equation 25
\begin{dmath}
1={ m_s _{t+1}}\, {R^s_{t}}
\end{dmath}
% Equation 26
\begin{dmath}
1={ m_REP _{t+1}}\, { R^{REP}_{Euler} _{t}}
\end{dmath}
% Equation 27
\begin{dmath}
1={ m_b _{t+1}}\, { R^b_{Euler} _{t}}
\end{dmath}
% Equation 28
\begin{dmath}
1={ R_k _{t}}\, { m_b _{t+1}}
\end{dmath}
% Equation 29
\begin{dmath}
{ \Theta _{t}}={K2Cltr\_BAR_{t}}^{1-{rho\_K2Cltr}}\, { \Theta _{t-1}}^{{rho\_K2Cltr}}
\end{dmath}
% Equation 30
\begin{dmath}
{ \bar{b^{b*}} _{t}}={K2Cltr\_f_{t}}\, {K2f_{t}}\, {K\_b\_BAR}
\end{dmath}
% Equation 31
\begin{dmath}
{ \bar{b} _{t}}={ \Theta _{t}}\, \left({K\_b\_BAR}\, { Constant Borrowing Limit }+\left(1-{ Constant Borrowing Limit }\right)\, \left({ Q_k _{t+1}}\, \left(1-{ Borrowing Limit without Capital  Price }\right)\, {K_b_{t+1}}+{ Borrowing Limit without Capital  Price }\, {K_b_{t+1}}\right)-{K2f_{t}}\, {K\_b\_BAR}\right)
\end{dmath}
% Equation 32
\begin{dmath}
{ \bar{b^{s*}} _{t}}=\left(-{b^s_{t}}\right)\, {Depo2Cltr\_f_{t}}
\end{dmath}
% Equation 33
\begin{dmath}
{Spread_R_b_{t}}=exp\left({\phi_{local}}\, \left(\frac{{b^b_{t}}}{{ \bar{b} _{t}}}-1\right)\right)\, {Shock to Spread R_b_{t}}
\end{dmath}
% Equation 34
\begin{dmath}
{Shock to Spread R_b_{t}}={Shock to Spread R_b_{t-1}}^{{\rho(e^{Spread}) }}\, exp\left({e\_Spread_{t}}\, {\sigma(e^{Spread}) }\right)
\end{dmath}
% Equation 35
\begin{dmath}
{R^b_{t}}={R^s_{t}}\, {Spread_R_b_{t}}
\end{dmath}
% Equation 36
\begin{dmath}
{ R^b_{Euler} _{t}}={R^b_{t}}\, exp\left(\left(\frac{{b^b_{t}}}{{ \bar{b} _{t}}}-1\right)\, {\nu }\right)
\end{dmath}
% Equation 37
\begin{dmath}
{R^{b*}_{t}}={R^b_{t}}
\end{dmath}
% Equation 38
\begin{dmath}
{b^{b*}_{t}}=0
\end{dmath}
% Equation 39
\begin{dmath}
{R^{s*}_{t}}={R^s_{t}}
\end{dmath}
% Equation 40
\begin{dmath}
{b^{s*}_{t}}=0
\end{dmath}
% Equation 41
\begin{dmath}
{Y\_prod_{t}}={Z_{t}}\, {K_{t}}^{{\alpha }}\, {L_{t}}^{1-{\alpha }}
\end{dmath}
% Equation 42
\begin{dmath}
{K/L_{t}}=\frac{{K_{t}}}{{L_{t}}}
\end{dmath}
% Equation 43
\begin{dmath}
{K/L_{t}}=\frac{{w_{t}}\, \frac{{\alpha }}{1-{\alpha }}}{{q_{t}}}
\end{dmath}
% Equation 44
\begin{dmath}
{L_{t}}={\chi^b }\, {L^b_{t}}+{L^s_{t}}\, {chi\_s}
\end{dmath}
% Equation 45
\begin{dmath}
{K_{t}}={\chi^b }\, {K_b_{t}}
\end{dmath}
% Equation 46
\begin{dmath}
{Y_{t}}={\chi^b }\, {Y^b_{t}}+{Y^s_{t}}\, {chi\_s}
\end{dmath}
% Equation 47
\begin{dmath}
{C_{t}}={\chi^b }\, {C^b_{t}}+{C^s_{t}}\, {chi\_s}
\end{dmath}
% Equation 48
\begin{dmath}
{I_{t}}={\chi^b }\, {I^b_{t}}
\end{dmath}
% Equation 49
\begin{dmath}
{I_{AC}_{t}}={\chi^b }\, {I_{AC}^b_{t}}
\end{dmath}
% Equation 50
\begin{dmath}
{\chi^b }\, {b^b_{t}}+{chi\_s}\, {b^s_{t}}=0
\end{dmath}
% Equation 51
\begin{dmath}
{TB_{t}}={\chi^b }\, {TB^b_{t}}+{TB^s_{t}}\, {chi\_s}
\end{dmath}
% Equation 52
\begin{dmath}
{Y_{t}}={TB_{t}}+{C_{t}}+{I_{t}}\, \left(1+{I_{AC}_{t}}\right)
\end{dmath}
% Equation 53
\begin{dmath}
{Y_{t}}={Y\_prod_{t}}
\end{dmath}
% Equation 54
\begin{dmath}
{ R^s_{nom}_{t}}={R^s_{t}}\, { E[\Pi]^{s} _{t}}
\end{dmath}
% Equation 55
\begin{dmath}
{ R^s_{nom}_{t}}={ R^{REP}_{Euler} _{t}}\, { E[\Pi]^{REP} _{t}}
\end{dmath}
% Equation 56
\begin{dmath}
{ E[\Pi] _{t}}={ E[\Pi]^{s} _{t}}
\end{dmath}
% Equation 57
\begin{dmath}
{ E[\Pi] _{t}}={ \Pi _{t+1}}
\end{dmath}
% Equation 58
\begin{dmath}
{ R^b_{nom}_{t}}={R^b_{t}}\, { E[\Pi] _{t}}
\end{dmath}
% Equation 59
\begin{dmath}
{ \pi _{t}}-\left({ \bar{\Pi} }-1\right)={\kappa}\, { \hat{MC} _{t}}+{beta\_b}\, \left({ E[\Pi] _{t}}-{ \bar{\Pi} }\right)
\end{dmath}
% Equation 60
\begin{dmath}
{Z_{t}}={Z\_BAR}^{1-{ \rho(e^Z) }}\, {Z_{t-1}}^{{ \rho(e^Z) }}\, exp\left({e\_Z_{t}}\, { \sigma(e^Z) }\right)
\end{dmath}
% Equation 61
\begin{dmath}
{MC_{t}}=\left(\frac{{q_{t}}}{{\alpha }}\right)^{{\alpha }}\, \left(\frac{{w_{t}}}{1-{\alpha }}\right)^{1-{\alpha }}\, \frac{1}{{Z_{t}}}
\end{dmath}
% Equation 62
\begin{dmath}
{ r_{Taylor} _{t}}={ExoZeroRate_{t}}\, \left({ \bar{\Pi} }-1+{R\_s\_SS}-1+\left({ \pi _{t}}-\left({ \bar{\Pi} }-1\right)\right)\, {\phi_{\pi}}+{\phi_{y}}\, { \hat{y} _{t}}\right)
\end{dmath}
% Equation 63
\begin{dmath}
{ r_{Taylor}^{NEW} _{t}}={ExoZeroRate_{t}}\, \left({ \bar{\Pi} }-1+{R\_s\_SS}-1+\left({ \pi _{t}}-\left({ \bar{\Pi} }-1\right)\right)\, {\phi_{\pi}}+{\phi_{y}}\, { \hat{y} - \tilde{y} _{t}}\right)
\end{dmath}
% Equation 64
\begin{dmath}
{ r^{CB}_{nom}_{t}}=max({ZLB\_min},{ r_{Taylor}^{NEW} _{t}})
\end{dmath}
% Equation 65
\begin{dmath}
{ Risk Premium Shock _{t}}={p\_R\_rp}^{1-{\rho(e^{RP}) }}\, { Risk Premium Shock _{t-1}}^{{\rho(e^{RP}) }}\, exp\left({e\_R\_rp_{t}}\, {\sigma(e^{RP}) }\right)
\end{dmath}
% Equation 66
\begin{dmath}
{ R^s_{nom}_{t}}={ Risk Premium Shock _{t}}\, \left(1+{ r^{CB}_{nom}_{t}}\right)
\end{dmath}
% Equation 67
\begin{dmath}
{ r^n _{t}}={R\_s\_SS}-1-{\chi^b }\, \left(exp\left(\left(\frac{{b^b_{t}}}{{ \bar{b} _{t}}}-1\right)\, \left({\phi_{local}}+{\nu }\right)\right)-1\right)
\end{dmath}
% Equation 68
\begin{dmath}
{r^n_{implied}_{t}}={R\_s\_SS}-1+\frac{{C_{t}}-{C_{t+1}}}{{sigma\_b}\, \left({\chi^b }\, {C\_b\_BAR\_l}+{chi\_s}\, {C\_s\_BAR\_l}\right)}+\frac{{ R^s_{nom}_{t}}}{{R\_s\_nom\_SS}}-1-\left({ \pi _{t+1}}-\left({ \bar{\Pi} }-1\right)\right)
\end{dmath}
% Equation 69
\begin{dmath}
{\Pi^Y_{t}}={Y\_prod_{t}}-\left({w_{t}}\, {L_{t}}+{K_{t}}\, {q_{t}}\right)
\end{dmath}
% Equation 70
\begin{dmath}
{Yb\_diff_{t}}={TB^b_{t}}+{DB^b_{t}}+{C^b_{t}}+{ Q_k _{t}}\, {I^b_{t}}-{w_{t}}\, {L^b_{t}}-{K_b_{t}}\, {q_{t}}
\end{dmath}
% Equation 71
\begin{dmath}
{w\_diff_{t}}={MC_{t}}\, {Z_{t}}\, \left(1-{\alpha }\right)\, {K/L_{t}}^{{\alpha }}-{w_{t}}
\end{dmath}
% Equation 72
\begin{dmath}
{delta\_Check_{t}}={Y_{t}}-{C_{t}}-{ Q_k _{t}}\, {I_{t}}-{TB_{t}}
\end{dmath}
% Equation 73
\begin{dmath}
{r^s_{t}}={R^s_{t}}-1
\end{dmath}
% Equation 74
\begin{dmath}
{r^b_{t}}={R^b_{t}}-1
\end{dmath}
% Equation 75
\begin{dmath}
{r^{s*}_{t}}={R^{s*}_{t}}-1
\end{dmath}
% Equation 76
\begin{dmath}
{r^{b*}_{t}}={R^{b*}_{t}}-1
\end{dmath}
% Equation 77
\begin{dmath}
{ r^s_{nom}_{t}}={ R^s_{nom}_{t}}-1
\end{dmath}
% Equation 78
\begin{dmath}
{ r^b_{nom}_{t}}={ R^b_{nom}_{t}}-1
\end{dmath}
% Equation 79
\begin{dmath}
{ \pi _{t}}={ \Pi _{t}}-1
\end{dmath}
% Equation 80
\begin{dmath}
{ \hat{y} _{t}}=\frac{{Y_{t}}}{{Y\_BAR}}-1
\end{dmath}
% Equation 81
\begin{dmath}
{ \hat{y} - \tilde{y} _{t}}={ \hat{y} _{t}}-{y\_tilde_{t}}
\end{dmath}
% Equation 82
\begin{dmath}
{ \hat{MC} _{t}}=\frac{{MC_{t}}}{{MC\_BAR}}-1
\end{dmath}
% Equation 83
\begin{dmath}
{\Pi^{foreign}_{banks}(b)_{t}}={b^{b*}_{t}}\, \left(\frac{1}{{R\_world}}-\frac{1}{{R^{b*}_{t}}}\right)
\end{dmath}
% Equation 84
\begin{dmath}
{\Pi^{foreign}_{banks}(s)_{t}}={b^{s*}_{t}}\, \left(\frac{1}{{R\_world}}-\frac{1}{{R^{s*}_{t}}}\right)
\end{dmath}
% Equation 85
\begin{dmath}
{\Pi^{foreign}_{banks}_{t}}={\chi^b }\, {\Pi^{foreign}_{banks}(b)_{t}}+{chi\_s}\, {\Pi^{foreign}_{banks}(s)_{t}}
\end{dmath}
% Equation 86
\begin{dmath}
{ C_s / C  _{t}}=\frac{{C^s_{t}}}{{C_{t}}}
\end{dmath}
% Equation 87
\begin{dmath}
{ NetWorth_b _{t}}={K_b_{t}}\, { Q_k _{t}}-{b^b_{t}}-{b^{b*}_{t}}
\end{dmath}
% Equation 88
\begin{dmath}
{ b^b / (Q * K^b) _{t}}=\frac{{b^b_{t}}}{{K_b_{t}}\, { Q_k _{t}}}
\end{dmath}
% Equation 89
\begin{dmath}
{ b / Y^B_{ann.} _{t}}=\frac{{b^b_{t}}}{{Y^b_{t}}\, 4}
\end{dmath}
% Equation 90
\begin{dmath}
{ b^{B*}/ Y_{ann.} _{t}}=\frac{{\chi^b }\, {b^{b*}_{t}}}{{Y_{t}}\, 4}
\end{dmath}
% Equation 91
\begin{dmath}
{b/ Y_{ann.} _{t}}=\frac{{\chi^b }\, {b^b_{t}}}{{Y_{t}}\, 4}
\end{dmath}
% Equation 92
\begin{dmath}
{r^s_{ann.}_{t}}={r^s_{t}}\, 4
\end{dmath}
% Equation 93
\begin{dmath}
{r^{s*}_{ann.}_{t}}={r^{s*}_{t}}\, 4
\end{dmath}
% Equation 94
\begin{dmath}
{r^b_{ann.}_{t}}={r^b_{t}}\, 4
\end{dmath}
% Equation 95
\begin{dmath}
{r^{b*}_{ann.}_{t}}={r^{b*}_{t}}\, 4
\end{dmath}
% Equation 96
\begin{dmath}
{ r^{REP.Euler}_{ann.} _{t}}=4\, \left({ R^{REP}_{Euler} _{t}}-1\right)
\end{dmath}
% Equation 97
\begin{dmath}
{ (r_b - r_s)_{ann.} _{t}}=4\, \left({Spread_R_b_{t}}-1\right)
\end{dmath}
% Equation 98
\begin{dmath}
{ (r_k - r_s)_{ann.} _{t}}=4\, \left(\frac{{ R_k _{t}}}{{R^s_{t}}}-1\right)
\end{dmath}
% Equation 99
\begin{dmath}
{ i_{ann.}_{t}}={ r^{CB}_{nom}_{t}}\, 4
\end{dmath}
% Equation 100
\begin{dmath}
{ r^s_{nom.ann.}_{t}}={ r^s_{nom}_{t}}\, 4
\end{dmath}
% Equation 101
\begin{dmath}
{ r^{RP}_{ann.}_{t}}=4\, \left({ Risk Premium Shock _{t}}-1\right)
\end{dmath}
% Equation 102
\begin{dmath}
{Shock to spread r_b ann._{t}}=4\, \left({Shock to Spread R_b_{t}}-1\right)
\end{dmath}
% Equation 103
\begin{dmath}
{ r^b_{nom.ann.}_{t}}={ r^b_{nom}_{t}}\, 4
\end{dmath}
% Equation 104
\begin{dmath}
{ \pi_{ann.} _{t}}={ \pi _{t}}\, 4
\end{dmath}
% Equation 105
\begin{dmath}
{ r^{b.Euler}_{ann.} _{t}}=4\, \left({ R^b_{Euler} _{t}}-1\right)
\end{dmath}
% Equation 106
\begin{dmath}
{ E[\pi]_{ann.} _{t}}=4\, \left({ E[\Pi] _{t}}-1\right)
\end{dmath}
% Equation 107
\begin{dmath}
{ E[\pi]_{ann.}^{s} _{t}}=4\, \left({ E[\Pi]^{s} _{t}}-1\right)
\end{dmath}
% Equation 108
\begin{dmath}
{ E[\pi]_{ann.}^{REP} _{t}}=4\, \left({ E[\Pi]^{REP} _{t}}-1\right)
\end{dmath}
% Equation 109
\begin{dmath}
{ r^k_{ann.} _{t}}=4\, \left({ R_k _{t}}-1\right)
\end{dmath}
