\documentclass[10pt,a4paper]{article}
\usepackage[landscape]{geometry}
\usepackage{fullpage}
\usepackage{breqn}
\begin{document}
\footnotesize
\begin{dmath}
% Equation 1
Y^s_{t}=C^s_{t}+DB^b_{t}+TB^s_{t}
\end{dmath}
\begin{dmath}
% Equation 2
Y^s_{t}=w_{t}\, L^s_{t}+\Pi^{local}_{banks}_{t}+ Gift From Borrowers _{t}
\end{dmath}
\begin{dmath}
% Equation 3
 Gift From Borrowers _{t}=\frac{\chi^b \,  NetWorth_b _{t}}{chi\_s}\, \left( Net Worth Shock _{t}-1\right)
\end{dmath}
\begin{dmath}
% Equation 4
 Net Worth Shock _{t}= Net Worth Shock _{t-1}^{\rho(e^NW) }\, exp\left(e\_NW_{t}\, \sigma(e^NW) \right)
\end{dmath}
\begin{dmath}
% Equation 5
\Pi^{local}_{banks}_{t}=\left(-b^s_{t}\right)\, \left(\frac{1}{R^s_{t}}-\frac{1}{R^b_{t}}\right)
\end{dmath}
\begin{dmath}
% Equation 6
DB^b_{t}=b^b_{t-1}-\frac{b^b_{t}}{R^b_{t}}
\end{dmath}
\begin{dmath}
% Equation 7
DB^b_{t}=b^s_{t-1}-\frac{b^s_{t}}{R^s_{t}}
\end{dmath}
\begin{dmath}
% Equation 8
TB^b_{t}=b^{b*}_{t-1}-\frac{b^{b*}_{t}}{R^{b*}_{t}}
\end{dmath}
\begin{dmath}
% Equation 9
TB^s_{t}=b^{s*}_{t-1}-\frac{b^{s*}_{t}}{R^{s*}_{t}}
\end{dmath}
\begin{dmath}
% Equation 10
\delta _{t}= p \delta ^{1- \rho(e^{\delta}) }\, \delta _{t-1}^{ \rho(e^{\delta}) }\, exp\left(e\_delta_{t}\,  \sigma(e^{\delta}) \right)
\end{dmath}
\begin{dmath}
% Equation 11
K_b_{t}=I^b_{t-1}+\left(1-\delta _{t}\right)\, K_b_{t-1}
\end{dmath}
\begin{dmath}
% Equation 12
\{mu}^b_{t}=\left(C^b_{t}-h^b \, C^b_{t-1}\right)^{\left(-sigma\_b\right)}-h^b \, beta\_b\, \left(C^b_{t+1}-C^b_{t}\, h^b \right)^{\left(-sigma\_b\right)}
\end{dmath}
\begin{dmath}
% Equation 13
\{mu}^s_{t}=\left(C^s_{t}-h^s \, C^s_{t-1}\right)^{\left(-\sigma_s\right)}-h^s \, \beta_s\, \left(C^s_{t+1}-C^s_{t}\, h^s \right)^{\left(-\sigma_s\right)}
\end{dmath}
\begin{dmath}
% Equation 14
\{mu}^{REP}_{t}=\left(C_{t}-h^s \, C_{t-1}\right)^{\left(-\sigma_s\right)}-h^s \, \beta_s\, \left(C_{t+1}-h^s \, C_{t}\right)^{\left(-\sigma_s\right)}
\end{dmath}
\begin{dmath}
% Equation 15
w_{t}=\frac{\vartheta^b\, L^b_{t}^{\omega^b }}{\{mu}^b_{t}}
\end{dmath}
\begin{dmath}
% Equation 16
w_{t}=\frac{\vartheta^s\, L^s_{t}^{\omega^s }}{\{mu}^s_{t}}
\end{dmath}
\begin{dmath}
% Equation 17
 m_b _{t}=\frac{\{mu}^b_{t}\, beta\_b}{\{mu}^b_{t-1}}
\end{dmath}
\begin{dmath}
% Equation 18
 m_s _{t}=\frac{\{mu}^s_{t}\, \beta_s}{\{mu}^s_{t-1}}
\end{dmath}
\begin{dmath}
% Equation 19
 m_REP _{t}=\frac{\beta_s\, \{mu}^{REP}_{t}}{\{mu}^{REP}_{t-1}}
\end{dmath}
\begin{dmath}
% Equation 20
 R_k _{t}=\frac{q_{t+1}+\left(1-\delta _{t}\right)\,  Q_k _{t+1}}{ Q_k _{t}}
\end{dmath}
\begin{dmath}
% Equation 21
I_{AC}_{t}=\frac{\gamma_2_b}{2}\, \left(\frac{I_{t}}{I_{t-1}}-1\right)^{2}
\end{dmath}
\begin{dmath}
% Equation 22
I_{MC}_{t}=\gamma_2_b\, \left(\frac{I_{t}}{I_{t-1}}-1\right)
\end{dmath}
\begin{dmath}
% Equation 23
 R_i _{t}=\frac{1}{beta\_b}
\end{dmath}
\begin{dmath}
% Equation 24
 Q_k _{t}=1+I_{AC}_{t}+\frac{I_{t}}{I_{t-1}}\, I_{MC}_{t}- m_b _{t+1}\, I_{MC}_{t+1}\, \left(\frac{I_{t+1}}{I_{t}}\right)^{2}
\end{dmath}
\begin{dmath}
% Equation 25
1=R^s_{t}\,  m_s _{t+1}
\end{dmath}
\begin{dmath}
% Equation 26
1= m_REP _{t+1}\,  R^{REP}_{Euler} _{t}
\end{dmath}
\begin{dmath}
% Equation 27
1= m_b _{t+1}\,  R^b_{Euler} _{t}
\end{dmath}
\begin{dmath}
% Equation 28
1= R_k _{t}\,  m_b _{t+1}
\end{dmath}
\begin{dmath}
% Equation 29
 \Theta _{t}=K2Cltr\_BAR_{t}^{1-rho\_K2Cltr}\,  \Theta _{t-1}^{rho\_K2Cltr}
\end{dmath}
\begin{dmath}
% Equation 30
 \bar{b^{b*}} _{t}=K2Cltr\_f_{t}\, K2f_{t}\, K\_b\_BAR
\end{dmath}
\begin{dmath}
% Equation 31
 \bar{b} _{t}= \Theta _{t}\, \left(K\_b\_BAR\,  Constant Borrowing Limit +\left(1- Constant Borrowing Limit \right)\, \left( Q_k _{t+1}\, \left(1- Borrowing Limit without Capital  Price \right)\, K_b_{t+1}+ Borrowing Limit without Capital  Price \, K_b_{t+1}\right)-K2f_{t}\, K\_b\_BAR\right)
\end{dmath}
\begin{dmath}
% Equation 32
 \bar{b^{s*}} _{t}=\left(-b^s_{t}\right)\, Depo2Cltr\_f_{t}
\end{dmath}
\begin{dmath}
% Equation 33
Spread_R_b_{t}=\left(1+\phi_{local}\, \left(\frac{b^b_{t}}{ \bar{b} _{t}}-1\right)\right)\, Shock to Spread R_b_{t}
\end{dmath}
\begin{dmath}
% Equation 34
Shock to Spread R_b_{t}=Shock to Spread R_b_{t-1}^{\rho(e^{Spread}) }\, exp\left(e\_Spread_{t}\, \sigma(e^{Spread}) \right)
\end{dmath}
\begin{dmath}
% Equation 35
R^b_{t}=R^s_{t}\, Spread_R_b_{t}
\end{dmath}
\begin{dmath}
% Equation 36
 R^b_{Euler} _{t}=R^b_{t}\, \left(1+\left(\frac{b^b_{t}}{ \bar{b} _{t}}-1\right)\, \nu \right)
\end{dmath}
\begin{dmath}
% Equation 37
R^{b*}_{t}=R^b_{t}
\end{dmath}
\begin{dmath}
% Equation 38
b^{b*}_{t}=0
\end{dmath}
\begin{dmath}
% Equation 39
R^{s*}_{t}=R^s_{t}
\end{dmath}
\begin{dmath}
% Equation 40
b^{s*}_{t}=0
\end{dmath}
\begin{dmath}
% Equation 41
Y\_prod_{t}=Z_{t}\, K_{t}^{\alpha }\, L_{t}^{1-\alpha }
\end{dmath}
\begin{dmath}
% Equation 42
K/L_{t}=\frac{K_{t}}{L_{t}}
\end{dmath}
\begin{dmath}
% Equation 43
K/L_{t}=\frac{w_{t}\, \frac{\alpha }{1-\alpha }}{q_{t}}
\end{dmath}
\begin{dmath}
% Equation 44
L_{t}=\chi^b \, L^b_{t}+L^s_{t}\, chi\_s
\end{dmath}
\begin{dmath}
% Equation 45
K_{t}=\chi^b \, K_b_{t}
\end{dmath}
\begin{dmath}
% Equation 46
Y_{t}=\chi^b \, Y^b_{t}+Y^s_{t}\, chi\_s
\end{dmath}
\begin{dmath}
% Equation 47
C_{t}=\chi^b \, C^b_{t}+C^s_{t}\, chi\_s
\end{dmath}
\begin{dmath}
% Equation 48
I_{t}=\chi^b \, I^b_{t}
\end{dmath}
\begin{dmath}
% Equation 49
I_{AC}_{t}=\chi^b \, I_{AC}^b_{t}
\end{dmath}
\begin{dmath}
% Equation 50
\chi^b \, b^b_{t}+chi\_s\, b^s_{t}=0
\end{dmath}
\begin{dmath}
% Equation 51
TB_{t}=\chi^b \, TB^b_{t}+TB^s_{t}\, chi\_s
\end{dmath}
\begin{dmath}
% Equation 52
Y_{t}=TB_{t}+C_{t}+ Q_k _{t}\, I_{t}
\end{dmath}
\begin{dmath}
% Equation 53
Y_{t}=Y\_prod_{t}
\end{dmath}
\begin{dmath}
% Equation 54
 R^s_{nom}_{t}=R^s_{t}\,  E[\Pi]^{s} _{t}
\end{dmath}
\begin{dmath}
% Equation 55
 R^s_{nom}_{t}= R^{REP}_{Euler} _{t}\,  E[\Pi]^{REP} _{t}
\end{dmath}
\begin{dmath}
% Equation 56
 E[\Pi] _{t}= E[\Pi]^{s} _{t}
\end{dmath}
\begin{dmath}
% Equation 57
 E[\Pi] _{t}= \Pi _{t+1}
\end{dmath}
\begin{dmath}
% Equation 58
 R^b_{nom}_{t}=R^b_{t}\,  E[\Pi] _{t}
\end{dmath}
\begin{dmath}
% Equation 59
 \pi _{t}-\left( \bar{\Pi} -1\right)=\kappa\,  \hat{MC} _{t}+beta\_b\, \left( E[\Pi] _{t}- \bar{\Pi} \right)
\end{dmath}
\begin{dmath}
% Equation 60
Z_{t}=Z\_BAR^{1- \rho(e^Z) }\, Z_{t-1}^{ \rho(e^Z) }\, exp\left(e\_Z_{t}\,  \sigma(e^Z) \right)
\end{dmath}
\begin{dmath}
% Equation 61
MC_{t}=\left(\frac{q_{t}}{\alpha }\right)^{\alpha }\, \left(\frac{w_{t}}{1-\alpha }\right)^{1-\alpha }\, \frac{1}{Z_{t}}
\end{dmath}
\begin{dmath}
% Equation 62
 r_{Taylor} _{t}=ExoZeroRate_{t}\, \left( \bar{\Pi} -1+R\_s\_SS-1+\left( \pi _{t}-\left( \bar{\Pi} -1\right)\right)\, \phi_{\pi}+\phi_{y}\,  \hat{y} _{t}\right)
\end{dmath}
\begin{dmath}
% Equation 63
 r_{Taylor}^{NEW} _{t}=ExoZeroRate_{t}\, \left( \bar{\Pi} -1+R\_s\_SS-1+\left( \pi _{t}-\left( \bar{\Pi} -1\right)\right)\, \phi_{\pi}+\phi_{y}\,  \hat{y} - \tilde{y} _{t}\right)
\end{dmath}
\begin{dmath}
% Equation 64
 r^{CB}_{nom}_{t}=max(ZLB\_min, r_{Taylor}^{NEW} _{t})
\end{dmath}
\begin{dmath}
% Equation 65
 Risk Premium Shock _{t}=p\_R\_rp^{1-\rho(e^{RP}) }\,  Risk Premium Shock _{t-1}^{\rho(e^{RP}) }\, exp\left(e\_R\_rp_{t}\, \sigma(e^{RP}) \right)
\end{dmath}
\begin{dmath}
% Equation 66
 R^s_{nom}_{t}= Risk Premium Shock _{t}\, \left(1+ r^{CB}_{nom}_{t}\right)
\end{dmath}
\begin{dmath}
% Equation 67
 r^n _{t}=R\_s\_SS-1-\left(\frac{b^b_{t}}{ \bar{b} _{t}}-1\right)\, \chi^b \, \left(\phi_{local}+\nu \right)
\end{dmath}
\begin{dmath}
% Equation 68
r^n_{implied}_{t}=R\_s\_SS-1+\frac{C_{t}-C_{t+1}}{sigma\_b\, \left(\chi^b \, C\_b\_BAR\_l+chi\_s\, C\_s\_BAR\_l\right)}+\frac{ R^s_{nom}_{t}}{R\_s\_nom\_SS}-1-\left( \pi _{t+1}-\left( \bar{\Pi} -1\right)\right)
\end{dmath}
\begin{dmath}
% Equation 69
\Pi^Y_{t}=Y\_prod_{t}-\left(w_{t}\, L_{t}+K_{t}\, q_{t}\right)
\end{dmath}
\begin{dmath}
% Equation 70
Yb\_diff_{t}=TB^b_{t}+DB^b_{t}+C^b_{t}+ Q_k _{t}\, I^b_{t}-w_{t}\, L^b_{t}-K_b_{t}\, q_{t}
\end{dmath}
\begin{dmath}
% Equation 71
w\_diff_{t}=MC_{t}\, Z_{t}\, \left(1-\alpha \right)\, K/L_{t}^{\alpha }-w_{t}
\end{dmath}
\begin{dmath}
% Equation 72
delta\_Check_{t}=Y_{t}-C_{t}- Q_k _{t}\, I_{t}-TB_{t}
\end{dmath}
\begin{dmath}
% Equation 73
r^s_{t}=R^s_{t}-1
\end{dmath}
\begin{dmath}
% Equation 74
r^b_{t}=R^b_{t}-1
\end{dmath}
\begin{dmath}
% Equation 75
r^{s*}_{t}=R^{s*}_{t}-1
\end{dmath}
\begin{dmath}
% Equation 76
r^{b*}_{t}=R^{b*}_{t}-1
\end{dmath}
\begin{dmath}
% Equation 77
 r^s_{nom}_{t}= R^s_{nom}_{t}-1
\end{dmath}
\begin{dmath}
% Equation 78
 r^b_{nom}_{t}= R^b_{nom}_{t}-1
\end{dmath}
\begin{dmath}
% Equation 79
 \pi _{t}= \Pi _{t}-1
\end{dmath}
\begin{dmath}
% Equation 80
 \hat{y} _{t}=\frac{Y_{t}}{Y\_BAR}-1
\end{dmath}
\begin{dmath}
% Equation 81
 \hat{y} - \tilde{y} _{t}= \hat{y} _{t}-y\_tilde_{t}
\end{dmath}
\begin{dmath}
% Equation 82
 \hat{MC} _{t}=\frac{MC_{t}}{MC\_BAR}-1
\end{dmath}
\begin{dmath}
% Equation 83
\Pi^{foreign}_{banks}(b)_{t}=b^{b*}_{t}\, \left(\frac{1}{R\_world}-\frac{1}{R^{b*}_{t}}\right)
\end{dmath}
\begin{dmath}
% Equation 84
\Pi^{foreign}_{banks}(s)_{t}=b^{s*}_{t}\, \left(\frac{1}{R\_world}-\frac{1}{R^{s*}_{t}}\right)
\end{dmath}
\begin{dmath}
% Equation 85
\Pi^{foreign}_{banks}_{t}=\chi^b \, \Pi^{foreign}_{banks}(b)_{t}+chi\_s\, \Pi^{foreign}_{banks}(s)_{t}
\end{dmath}
\begin{dmath}
% Equation 86
 C_s / C  _{t}=\frac{C^s_{t}}{C_{t}}
\end{dmath}
\begin{dmath}
% Equation 87
 NetWorth_b _{t}=K_b_{t}\,  Q_k _{t}-b^b_{t}-b^{b*}_{t}
\end{dmath}
\begin{dmath}
% Equation 88
 b^b / (Q * K^b) _{t}=\frac{b^b_{t}}{K_b_{t}\,  Q_k _{t}}
\end{dmath}
\begin{dmath}
% Equation 89
 b / Y^B_{ann.} _{t}=\frac{b^b_{t}}{Y^b_{t}\, 4}
\end{dmath}
\begin{dmath}
% Equation 90
 b^{B*}/ Y_{ann.} _{t}=\frac{\chi^b \, b^{b*}_{t}}{Y_{t}\, 4}
\end{dmath}
\begin{dmath}
% Equation 91
b/ Y_{ann.} _{t}=\frac{\chi^b \, b^b_{t}}{Y_{t}\, 4}
\end{dmath}
\begin{dmath}
% Equation 92
r^s_{ann.}_{t}=r^s_{t}\, 4
\end{dmath}
\begin{dmath}
% Equation 93
r^{s*}_{ann.}_{t}=r^{s*}_{t}\, 4
\end{dmath}
\begin{dmath}
% Equation 94
r^b_{ann.}_{t}=r^b_{t}\, 4
\end{dmath}
\begin{dmath}
% Equation 95
r^{b*}_{ann.}_{t}=r^{b*}_{t}\, 4
\end{dmath}
\begin{dmath}
% Equation 96
 r^{REP.Euler}_{ann.} _{t}=4\, \left( R^{REP}_{Euler} _{t}-1\right)
\end{dmath}
\begin{dmath}
% Equation 97
 (r_b - r_s)_{ann.} _{t}=4\, \left(Spread_R_b_{t}-1\right)
\end{dmath}
\begin{dmath}
% Equation 98
 (r_k - r_s)_{ann.} _{t}=4\, \left(\frac{ R_k _{t}}{R^s_{t}}-1\right)
\end{dmath}
\begin{dmath}
% Equation 99
 i_{ann.}_{t}= r^{CB}_{nom}_{t}\, 4
\end{dmath}
\begin{dmath}
% Equation 100
 r^s_{nom.ann.}_{t}= r^s_{nom}_{t}\, 4
\end{dmath}
\begin{dmath}
% Equation 101
 r^{RP}_{ann.}_{t}=4\, \left( Risk Premium Shock _{t}-1\right)
\end{dmath}
\begin{dmath}
% Equation 102
Shock to spread r_b ann._{t}=4\, \left(Shock to Spread R_b_{t}-1\right)
\end{dmath}
\begin{dmath}
% Equation 103
 r^b_{nom.ann.}_{t}= r^b_{nom}_{t}\, 4
\end{dmath}
\begin{dmath}
% Equation 104
 \pi_{ann.} _{t}= \pi _{t}\, 4
\end{dmath}
\begin{dmath}
% Equation 105
 r^{b.Euler}_{ann.} _{t}=4\, \left( R^b_{Euler} _{t}-1\right)
\end{dmath}
\begin{dmath}
% Equation 106
 E[\pi]_{ann.} _{t}=4\, \left( E[\Pi] _{t}-1\right)
\end{dmath}
\begin{dmath}
% Equation 107
 E[\pi]_{ann.}^{s} _{t}=4\, \left( E[\Pi]^{s} _{t}-1\right)
\end{dmath}
\begin{dmath}
% Equation 108
 E[\pi]_{ann.}^{REP} _{t}=4\, \left( E[\Pi]^{REP} _{t}-1\right)
\end{dmath}
\begin{dmath}
% Equation 109
 r^k_{ann.} _{t}=4\, \left( R_k _{t}-1\right)
\end{dmath}
\end{document}
